VariableDefinitions.v
@@ -1,0 +1,3 @@
+Require Export Coq.Strings.String.
+
+Definition var := string.
